commit

AP/Util/Data/Set.lean
@@ -5,6 +5,7 @@ universe u v w
 structure Set' (α : Type u)
 [hh₁ : DecidableEq α] [hh₂ : Hashable α] : Type u where
   inner : Std.ExtDHashMap α (λ _ => Unit)
+deriving Inhabited
 
 variable {α : Type u} {β : Type v} {γ : Type w}
 variable [ha₁ : DecidableEq α] [ha₂ : Hashable α]
@@ -21,8 +22,6 @@ def empty : Set' α := ⟨∅⟩
 instance : EmptyCollection (Set' α) := ⟨empty⟩
 
 theorem empty_def : (∅ : Set' α) = ⟨∅⟩ := rfl
-
-instance : Inhabited (Map α β) := ⟨∅⟩
 
 def insertP (x : α) (s : Set' α) : Set' α :=
   ⟨insert ⟨x, ()⟩ s.inner⟩
@@ -227,3 +226,96 @@ instance [ha : Finite α] : Finite (Set' α) := by
   apply Fintype.finite
   replace ha := @Fintype.ofFinite _ ha
   infer_instance
+
+def fold (s : Set' α) (z : β) (f : β → α → β)
+(h_assoc : ∀ {acc x y}, f (f acc x) y = f (f acc y) x) : β :=
+  s.inner.fold z (λ acc x _ => f acc x) # by simpa
+
+def fold₁ (s : Set' α) (f : α → α → α)
+(h_comm : ∀ {x y}, f x y = f y x)
+(h_assoc : ∀ {acc x y}, f (f acc x) y = f (f acc y) x) : Option α :=
+  s.fold none (λ acc x => some # acc.elim x (f · x)) # by
+    rintro (⟨⟩ | acc) x y <;> simp
+    exact h_comm; exact h_assoc
+
+def min? [ha : LinearOrder α] (s : Set' α) : Option α :=
+  s.fold₁ min (min_comm _ _) (inf_right_comm _ _ _)
+
+def max? [ha : LinearOrder α] (s : Set' α) : Option α :=
+  s.fold₁ max (max_comm _ _) (sup_right_comm _ _ _)
+
+def min! [ha : LinearOrder α] [Inhabited α] (s : Set' α) : α :=
+  s.min?.get!
+
+def max! [ha : LinearOrder α] [Inhabited α] (s : Set' α) : α :=
+  s.max?.get!
+
+theorem fold_eq_foldl_toList {β : Type*} [ha : LinearOrder α]
+{z : β} {f : β → α → β} {h_assoc} : s.fold z f h_assoc = s.toList.foldl f z := by
+  convert Std.ExtDHashMap.fold_eq_foldl_toList
+  rotate_left; infer_instance
+  rcases s with ⟨⟨mp⟩⟩
+  unfold Set'.toList Std.ExtDHashMap.toList Std.ExtDHashMap.lift
+    toSortedKeys toSortedList
+  apply mp.ind
+  intro m
+  simp
+  rw [List.foldl_map]
+
+theorem min?_eq_head?_toList [ha : LinearOrder α] : s.min? = s.toList.head? := by
+  rw [min?, fold₁, fold_eq_foldl_toList]
+  convert @s.toList.min?_eq_head? α _ _
+  rotate_left; simp_rw [min_eq_left_iff]; exact sorted_toList
+  ext:1; nm xs; cases xs <;> simp; nm x xs
+  apply List.foldl_some_some.trans
+  simp; rw [List.foldl_min]; cases xs.min? <;> simp
+
+theorem max?_eq_last?_toList [ha : LinearOrder α] : s.max? = s.toList.getLast? := by
+  rw [max?, fold₁, fold_eq_foldl_toList]
+  convert @s.toList.max?_eq_getLast? α _ _
+  rotate_left; exact sorted_toList
+  ext:1; nm xs; cases xs <;> simp; nm x xs
+  apply List.foldl_some_some.trans
+  simp; rw [List.foldl_max]; cases xs.max? <;> simp
+
+@[simp]
+theorem ofList_toList [ha : LinearOrder α] : ofList s.toList = s := by
+  ext; simp
+
+theorem ind_ofList [ha : LinearOrder α] {p : Set' α → Prop}
+(h : ∀ (xs : List α), xs.Nodup → xs.Sorted (· ≤ ·) → p (ofList xs))
+(s : Set' α) : p s := by rw [←ofList_toList (s := s)]; apply h <;> simp
+
+#check 0 #exit
+
+@[simp]
+theorem toList_ofList_perm [ha : LinearOrder α] {xs : List α}
+(h : xs.Nodup) : (ofList xs).toList.Perm xs := by
+  have h₁ := @Std.DHashMap.toList_ofList_perm
+  specialize @h₁ α (λ _ => Unit) _ _ (xs.map (⟨·, ()⟩)) (by simpa)
+  -- simp [ofList, toList, Std.ExtDHashMap.lift]
+  convert_to (((ofList xs).toList.map λ x =>
+    (⟨x, ()⟩ : (_ : α) × Unit)).map (·.1)).Perm ((xs.map # λ x =>
+    (⟨x, ()⟩ : (_ : α) × Unit)).map (·.1)); iterate 2 simp
+  rw [List.map_perm_map_iff_loc]
+  · convert h₁
+    symm
+    apply List.eq_of_perm_of_sorted_loc
+    · simp
+
+#check 0 #exit
+
+theorem toList_ofList [ha : LinearOrder α] {xs : List α}
+(h₁ : xs.Nodup) (h₂ : xs.Sorted (· ≤ ·)) : (ofList xs).toList = xs := by
+  apply List.eq_of_perm_of_sorted_loc
+  · exact?
+
+#check 0 #exit
+
+theorem not_mem_of_lt_min? [ha : LinearOrder α] {m x}
+(h₁ : s.min? = some m) (h₂ : x < m) : x ∉ s := by
+  induction s using ind_ofList; clear! s
+  nm xs h₃ h₄
+  simp [min?_eq_head?_toList] at h₁
+  convert_to xs.Pairwise (λ a b => min a b = a) at h₄; simp
+  have := List.min?_eq_head? h₄
