AP/AP/Basic.lean
@@ -1,0 +1,67 @@
+import AP.AP.Defs
+
+namespace AP
+
+theorem aStrat_valid_def {a : AStrat} : a.Valid ↔ ∀ {s} [sys.Valid s],
+sys.hasTr s → s.a_turn → sys.validTr s (a.f s) := ⟨λ ⟨h⟩ => h, λ h => ⟨h⟩⟩
+
+theorem dStrat_valid_def {d : DStrat} : d.Valid ↔ ∀ {s} [sys.Valid s],
+sys.hasTr s → s.a_turn = false → sys.validTr s (d.f s) := ⟨λ ⟨h⟩ => h, λ h => ⟨h⟩⟩
+
+theorem strat_valid_def {st : Strat} : st.Valid ↔ ∀ {s} [sys.Valid s],
+sys.hasTr s → sys.validTr s (st.f s) := ⟨λ ⟨h⟩ => h, λ h => ⟨h⟩⟩
+
+theorem strat_valid_iff {st : Strat} : st.Valid ↔ st.a.Valid ∧ st.d.Valid := by
+  rw [strat_valid_def, aStrat_valid_def, dStrat_valid_def]
+  simp [System.hasTr, System.validTr, Strat.f]
+  constructor
+  · intro h
+    constructor
+    all_goals
+      intro s hs p s' h₁ h₂
+      specialize h _ _ h₁
+      simp [h₂] at h
+      exact h
+  · rintro ⟨h₁, h₂⟩
+    intro s hs p s' h₃
+    split_ifs with h₄
+    · exact h₁ _ _ h₃ h₄
+    · simp at h₄; exact h₂ _ _ h₃ h₄
+
+theorem Strat.Valid.a_valid {st : Strat} [hst : st.Valid] : st.a.Valid := by
+  rw [strat_valid_iff] at hst; exact hst.1
+
+theorem Strat.Valid.d_valid {st : Strat} [hst : st.Valid] : st.d.Valid := by
+  rw [strat_valid_iff] at hst; exact hst.2
+
+instance {st : Strat} [hst : st.Valid] : st.a.Valid := hst.a_valid
+instance {st : Strat} [hst : st.Valid] : st.d.Valid := hst.d_valid
+
+abbrev State.Valid (s : State) : Prop := sys.Valid s
+
+@[class]
+structure State.AState (s : State) : Prop where
+  h_valid : s.Valid
+  h : s.a_turn
+
+@[class]
+structure State.DState (s : State) : Prop where
+  h_valid : s.Valid
+  h : s.a_turn = false
+
+theorem aState_def {s : State} : s.AState ↔ s.Valid ∧ s.a_turn :=
+  ⟨λ ⟨h₁, h₂⟩ => ⟨h₁, h₂⟩, λ ⟨h₁, h₂⟩ => ⟨h₁, h₂⟩⟩
+
+theorem dState_def {s : State} : s.DState ↔ s.Valid ∧ s.a_turn = false :=
+  ⟨λ ⟨h₁, h₂⟩ => ⟨h₁, h₂⟩, λ ⟨h₁, h₂⟩ => ⟨h₁, h₂⟩⟩
+
+#check 0 #exit
+
+@[simp]
+theorem State.DState.hasTr_iff {s : State} [hs : s.DState] : sys.hasTr s := by
+  rcases hs with ⟨hs, ht⟩
+  use s.taken.max + 1
+
+#check 0 #exit
+
+theorem d_has_move {s : State} [hs : s.DState] : sys.hasTr s := by
