AP/AP/Defs.lean
@@ -1,0 +1,87 @@
+import AP.Point
+import AP.System.Main
+
+namespace AP
+
+structure State : Type where
+  pw : ℕ
+  taken : Set' PointZ
+  a_pos : PointZ
+  a_turn : Bool
+  hist : List PointZ
+deriving Inhabited, DecidableEq
+
+structure AStrat : Type where
+  f : State → PointZ
+deriving Inhabited
+
+structure DStrat : Type where
+  f : State → PointZ
+deriving Inhabited
+
+structure Strat : Type where
+  a : AStrat
+  d : DStrat
+deriving Inhabited
+
+-----
+
+def state₀ (pw : ℕ) : State :=
+  { pw := pw
+  , taken := ∅
+  , a_pos := 0
+  , a_turn := false
+  , hist := []
+  }
+
+def State.a_move (s : State) (p : PointZ) : Option State := do
+  guard # s.a_pos ≠ p
+  guard # p ∉ s.taken
+  guard # p.dist s.a_pos ≤ s.pw
+  return {s with a_pos := p, a_turn := false}
+
+def State.d_move (s : State) (p : PointZ) : Option State := do
+  guard # s.a_pos ≠ p
+  guard # p ∉ s.taken
+  return {s with taken := insert p s.taken, a_turn := false}
+
+def State.move (s : State) (p : PointZ) : Option State :=
+  if s.a_turn then s.a_move p else s.d_move p
+
+def sys : System State PointZ :=
+  { initial := {s | ∃ pw, state₀ pw = s}
+  , tr := State.move
+  }
+
+@[class]
+structure AStrat.Valid (a : AStrat) : Prop where
+  h : ∀ {s} [sys.Valid s], sys.hasTr s → s.a_turn → sys.validTr s (a.f s)
+
+@[class]
+structure DStrat.Valid (d : DStrat) : Prop where
+  h : ∀ {s} [sys.Valid s], sys.hasTr s → s.a_turn = false → sys.validTr s (d.f s)
+
+def Strat.f (st : Strat) (s : State) : PointZ :=
+  if s.a_turn then st.a.f s else st.d.f s
+
+@[class]
+structure Strat.Valid (st : Strat) : Prop where
+  h : ∀ {s} [sys.Valid s], sys.hasTr s → sys.validTr s (st.f s)
+
+def State.a_wins (s : State) (st : Strat) : Prop :=
+  ∀ n, (sys.simulate st.f s n).2 = 0
+
+def State.d_wins (s : State) (st : Strat) : Prop :=
+  ¬s.a_wins st
+
+def State.a_hws (s : State) : Prop :=
+  ∃ (a : AStrat), a.Valid ∧ ∀ (d : DStrat), d.Valid → s.a_wins ⟨a, d⟩
+
+def State.d_hws (s : State) : Prop :=
+  ∃ (d : DStrat), d.Valid ∧ ∀ (a : AStrat), a.Valid → s.d_wins ⟨a, d⟩
+
+def a_hws_pw (pw : ℕ) : Prop :=
+  (state₀ pw).a_hws
+
+def d_hws_pw (pw : ℕ) : Prop :=
+  (state₀ pw).d_hws
